refactor: Make coq-prelude less opinionated
coq-prelude was initially an attempt to provide a more Haskell-flavor
API to Coq development. This has proven to be less effective than
anticipated in practice.

This patch is a first important step toward making coq-prelude less
opinionated. In particular:

  - We reuse existing type as much as possible (for instance, no more
    [Either], we use [sum] instead)
  - The monad notations form a compromise between the Haskell
    do-notation and OCaml 4.08 new “monadic” operators
  - We remove the [Integer] libraries

With this patch, the minimum Coq version to use coq-prelude is
coq.8.10.0.

theories/Control.v
@@ -15,208 +15,185 @@
  * along with this program. If not, see <http://www.gnu.org/licenses/>.
  *)
 
+From Coq Require Import Equivalence Setoid Morphisms.
+From Prelude Require Export Equality.
+
 Set Universe Polymorphism.
 
-Require Import Coq.Classes.Equivalence.
-Require Import Coq.Setoids.Setoid.
+Declare Scope monad_scope.
+Delimit Scope monad_scope with monad.
 
-Require Import Prelude.Equality.
+#[local]
+Open Scope prelude_scope.
 
-Local Open Scope prelude_scope.
+Definition compose {a b c} (g : b -> c) (f : a -> b) : a -> c :=
+  fun (x: a) => g (f x).
 
-Definition compose
-           {a b c:  Type}
-           (g:      b -> c)
-           (f:      a -> b)
-  : a -> c :=
-  fun (x: a)
-  => g (f x).
+Definition id {a : Type} (x : a) : a := x.
 
-Definition id
-           {a:  Type}
-           (x:  a)
-  : a :=
-  x.
+Notation "f <<< g" := (compose f g) (at level 50) : function_scope.
+Notation "f >>> g" := (compose g f) (at level 50) : function_scope.
 
-Notation "f <<< g" :=
-  (compose f g) (at level 50)
-  : prelude_scope.
-
-Notation "f >>> g" :=
-  (compose g f) (at level 50)
-  : prelude_scope.
+Notation "'fun*' x .. z '=>' p" := (fun x => .. (fun z => p%monad) ..)
+  (x binder, z binder, at level 200, only parsing) : function_scope.
 
 Notation "f $ x" :=
-  (f x) (only parsing, at level 99, right associativity)
-  : prelude_scope.
+  (f x) (only parsing, at level 99, right associativity) : prelude_scope.
 
-(** * Functor
+(** * Functor *)
 
- *)
+Class Functor (f : Type -> Type) : Type :=
+  { functor_has_eq :> forall {a} `{Equality a}, Equality (f a)
+  ; map {a b : Type} : (a -> b) -> f a -> f b
+  ; functor_identity {a} `{Equality a} (x : f a) : map id x == id x
+  ; functor_map_identity {a b c} `{Equality c} (u : b -> c) (v : a -> b) (x : f a)
+    : map (u <<< v) x == map u (map v x)
+  }.
 
-Class Functor
-      (f:  Type -> Type)
-  := { functor_has_eq :> forall {a: Type}
-                               `{Equality a},
-           Equality (f a)
-     ; map {a b: Type}
-           (g:   a -> b)
-           (x:   f a)
-       : f b
-     ; functor_identity {a: Type} `{Equality a}
-                        (x: f a)
-       : map (@id a) x == id x
-     ; functor_composition_identity {a b c:  Type} `{Equality c}
-                                    (u:      b -> c)
-                                    (v:      a -> b)
-                                    (x:      f a)
-       : map (u <<< v) x == ((map u) <<< (map v)) x
-     }.
-
-Arguments map [f _ a b] (_ _).
+Arguments map [f _ a b] (_ _%monad).
 Arguments functor_identity [f _ a _] (x).
-Arguments functor_composition_identity [f _ a b c _] (u v x).
+Arguments functor_map_identity [f _ a b c _] (u v x).
 
-Notation "f <$> g" :=
-  (map f g) (at level 27, left associativity)
-  : prelude_scope.
+Definition fconst {f a b} `{Functor f} (x : a) (ft : f b) : f a :=
+  map (fun _ => x) ft.
 
-(** * Applicative
+Arguments fconst [f a b _] x ft%monad.
 
- *)
+Notation "f <$> g" := (map f g) (at level 27, left associativity) : monad_scope.
+Notation "f <$ g" := (fconst f g) (at level 27, left associativity) : monad_scope.
+
+#[local]
+Open Scope monad_scope.
+
+(** * Applicative *)
 
 Reserved Notation "f <*> g" (at level 28, left associativity).
 
-Class Applicative
-      (f:  Type -> Type)
-  := { applicative_is_functor :> Functor f
-     ; pure {a:  Type}
-       : a -> f a
-     ; apply {a b:  Type}
-       : f (a -> b)
-         -> f a
-         -> f b
-       where "f <*> g" := (apply f g)
-     ; applicative_identity {a:  Type} `{Equality a}
-                            (v:  f a)
-       : pure id <*> v == v
-     ; applicative_composition {a b c:  Type} `{Equality c}
-                               (u:      f (b -> c))
-                               (v:      f (a -> b))
-                               (w:      f a)
-       : pure compose <*> u <*> v <*> w == u <*> (v <*> w)
-     ; applicative_homomorphism {a b:  Type} `{Equality b}
-                                (v:    a -> b)
-                                (x:    a)
-       : (pure v) <*> (pure x) == pure (v x)
-     ; applicative_interchange {a b:  Type} `{Equality b}
-                               (u:    f (a -> b))
-                               (y:    a)
-       : u <*> (pure y) == (pure (fun z => z y)) <*> u
-     ; applicative_pure_map {a b: Type} `{Equality b}
-                            (g: a -> b)
-                            (x: f a)
-       : g <$> x == pure g <*> x
-     }.
-
-Notation "f <*> g" :=
-  (apply f g)
-    (at level 28, left associativity)
-  : prelude_scope.
+Class Applicative (f : Type -> Type) : Type :=
+  { applicative_is_functor :> Functor f
+  ; pure {a} : a -> f a
+  ; apply {a b} : f (a -> b) -> f a -> f b
+    where "f <*> g" := (apply f g)
+  ; applicative_identity {a} `{Equality a} (v : f a) : pure id <*> v == v
+  ; applicative_composition {a b c} `{Equality c} (u : f (b -> c)) (v : f (a -> b)) (w : f a)
+    : pure compose <*> u <*> v <*> w == u <*> (v <*> w)
+  ; applicative_homomorphism {a b} `{Equality b} (v : a -> b) (x : a)
+    : (pure v) <*> (pure x) == pure (v x)
+  ; applicative_interchange {a b} `{Equality b} (u : f (a -> b)) (y : a)
+    : u <*> (pure y) == (pure (fun z => z y)) <*> u
+  ; applicative_pure_map {a b} `{Equality b} (g : a -> b) (x : f a)
+    : g <$> x == pure g <*> x
+  }.
 
 Arguments pure [f _ a] (x).
-Arguments apply [f _ a b] (_ _).
+Arguments apply [f _ a b] (_%monad _%monad).
 Arguments applicative_identity [f _ a _] (v).
 Arguments applicative_composition [f _ a b c _] (u v w).
 Arguments applicative_homomorphism [f _ a b _] (v x).
 Arguments applicative_interchange [f _ a b _] (u y).
 Arguments applicative_pure_map [f _ a b _] (g x).
 
-(** * Monad
+Notation "f <*> g" := (apply f g) (at level 28, left associativity) : monad_scope.
 
- *)
+Definition liftA2 {f a b c} `{Applicative f} (g : a -> b -> c) (x : f a) (y : f b) : f c :=
+  apply (map g x) y.
 
-Reserved Notation "f >>= g" (at level 28, left associativity).
+Arguments liftA2 [f a b c _] (g x%monad y%monad).
 
-Class Monad
-      (m:  Type -> Type)
-  := { monad_is_apply :> Applicative m
-     ; bind {a b:  Type}
-       : m a
-         -> (a -> m b)
-         -> m b
-       where "f >>= g" := (bind f g)
-     ; monad_left_identity {a b:  Type} `{Equality b}
-                           (x:    a)
-                           (f:    a -> m b)
-       : pure x >>= f == f x
-     ; monad_right_identity {a:  Type} `{Equality a}
-                            (x:  m a)
-       : x >>= (fun y => pure y) == x
-     ; monad_bind_associativity {a b c:  Type} `{Equality c}
-                                (f:      m a)
-                                (g:      a -> m b)
-                                (h:      b -> m c)
-       : (f >>= g) >>= h == f >>= (fun x => (g x) >>= h)
-     ; monad_bind_morphism {a b:   Type} `{Equality b}
-                           (x:     m a)
-                           (f f':  a -> m b)
-       : f == f' -> bind x f == bind x f'
-     ; monad_bind_map {a b:  Type} `{Equality b}
-                      (x:    m a)
-                      (f:    a -> b)
-       : f <$> x == (x >>= (fun y => pure (f y)))
-     }.
+Definition rseq {f a b} `{Applicative f} (x : f a) (y : f b) : f b :=
+  (id <$ x) <*> y.
 
-Arguments bind [m _ a b] (f g).
-Arguments monad_left_identity [m _ a b _] (x f).
-Arguments monad_right_identity [m _ a _] (x).
-Arguments monad_bind_associativity [m _ a b c _] (f g h).
-Arguments monad_bind_morphism [m _ a b _] (x f f').
-Arguments monad_bind_map [m _ a b _] (x f).
+Arguments rseq [f a b _] (x%monad y%monad).
 
-Add Parametric Morphism
-    (m:    Type -> Type) `{M: Monad m}
-    (a b:  Type) `{Equality a} `{B: Equality b}
-  : (@bind m M a b)
-    with signature (@eq (m a))
-                   ==> (@equal (a -> m b) _)
-                   ==> (@equal (m b) functor_has_eq)
-      as bind_morphism_decl.
-Proof.
-  intros x f f' Heq.
-  apply (monad_bind_morphism x f f' Heq).
+Notation "f *> g" := (rseq f g) (at level 28, left associativity) : monad_scope.
+
+Definition lseq {f a b} `{Applicative f} (x : f a) (y : f b) : f a :=
+  liftA2 (fun x _ => x) x y.
+
+Arguments lseq [f a b _] (x%monad y%monad).
+
+Notation "f <* g" := (lseq f g) (at level 28, left associativity) : monad_scope.
+
+(** * Monad *)
+
+Reserved Notation "f >>= g" (at level 20, left associativity).
+
+Class Monad (m:  Type -> Type) :=
+  { monad_is_apply :> Applicative m
+  ; bind {a b} : m a -> (a -> m b) -> m b
+    where "f >>= g" := (bind f g)
+  ; bind_left_identity {a b} `{Equality b} (x : a) (f : a -> m b)
+    : pure x >>= f == f x
+  ; bind_right_identity {a} `{Equality a} (x : m a)
+    : x >>= (fun y => pure y) == x
+  ; bind_associativity {a b c} `{Equality c} (f : m a) (g : a -> m b) (h : b -> m c)
+    : (f >>= g) >>= h == f >>= (fun x => (g x) >>= h)
+  ; bind_morphism {a b} `{Equality b} (x : m a) (f f' : a -> m b)
+    : f == f' -> bind x f == bind x f'
+  ; bind_map {a b} `{Equality b} (x : m a) (f : a -> b)
+    : f <$> x == (x >>= (fun y => pure (f y)))
+  }.
+
+Notation "f >>= g" := (bind f g) (at level 20, left associativity) : monad_scope.
+
+Arguments bind [m _ a b] (f%monad g%monad).
+Arguments bind_left_identity [m _ a b _] (x f).
+Arguments bind_right_identity [m _ a _] (x).
+Arguments bind_associativity [m _ a b c _] (f g h).
+Arguments bind_morphism [m _ a b _] (x f f').
+Arguments bind_map [m _ a b _] (x f).
+
+#[local]
+Open Scope signature_scope.
+
+#[program]
+Instance bind_Proper (m : Type -> Type) `{Monad m} (a b : Type) `{Equality b}
+  : Proper (@eq (m a) ==> @equal (a -> m b) _ ==> @equal (m b) functor_has_eq) (@bind m _ _ _).
+
+Next Obligation.
+  add_morphism_tactic.
+  intros x f g equ.
+  apply bind_morphism.
+  exact equ.
 Qed.
 
-Notation "f >>= g" := (bind f g) (at level 28, left associativity).
-
-Definition join
-           {m:  Type -> Type} `{Monad m}
-           {a:  Type}
-           (x:  m (m a))
-  : m a :=
+Definition join {m a} `{Monad m} (x : m (m a)) : m a :=
   x >>= id.
 
-Definition void
-           {m:  Type -> Type} `{Monad m}
-           {a:  Type}
-           (x:  m a)
-  : m unit :=
+Arguments join [m a _] (x%monad).
+
+Definition void {m a} `{Monad m} (x : m a) : m unit :=
   x >>= fun _ => pure tt.
 
-Definition when
-           {m:     Type -> Type} `{Monad m}
-           {a:     Type}
-           (cond:  bool)
-           (x:     m a)
-  : m unit :=
-  if cond
-  then void x
-  else pure tt.
+Arguments void [m a _] (x%monad).
 
-Notation "a <- p ; q" :=
-  (bind p (fun a => q)) (at level 100, right associativity, p at next level)
-  : prelude_scope.
-Notation "p ;; q" :=
-  (bind p (fun _ => q)) (at level 100, right associativity)
-  : prelude_scope.
+Definition when {m a} `{Monad m} (cond : bool) (x : m a) : m unit :=
+  if cond then void x else pure tt.
+
+Arguments when [m a _] (cond x%monad).
+
+Declare Custom Entry monad.
+
+Notation "'do' p 'end'" := p (p custom monad at level 10) : prelude_scope.
+
+Notation "p ';' q" := (bind p%monad (fun _ => q%monad))
+  (in custom monad at level 10, q at level 10, right associativity, only parsing).
+
+Notation "'let*' a '<-' p 'in' q" := (bind p%monad (fun a => q%monad))
+  (in custom monad at level 0, a ident, p constr, q at level 10, right associativity, only parsing).
+
+Notation "'let' a ':=' p 'in' q" := (let a := p in q%monad)
+  (in custom monad at level 5, a ident, p constr, q at level 10, right associativity, only parsing).
+
+Notation "x" := x%monad (in custom monad at level 0, x constr at level 200, only parsing).
+
+#[local]
+Definition test_monad_notation {m} `{Monad m}
+  (compute : nat -> m nat) (p : m unit) (q : nat -> m bool) : nat -> m bool := fun* _ => do
+    p >>= (fun _ => q 2%nat);
+    p;
+    let z := 3 in
+    let* x <- id <$> compute 3 in
+    let* y <- compute 4 in
+    q (x + y + z)
+  end.
