theories/Control/State.v
@@ -15,435 +15,276 @@
  * along with this program. If not, see <http://www.gnu.org/licenses/>.
  *)
 
+From Coq Require Import FunctionalExtensionality Program.Basics.
+From Prelude Require Import Control Classes Identity Equality.
+
 Set Universe Polymorphism.
 
-Require Import Coq.Logic.FunctionalExtensionality.
-Require Import Coq.Program.Basics.
+#[local]
+Close Scope nat_scope.
+#[local]
+Open Scope prelude_scope.
 
-Require Import Prelude.Control.
-Require Import Prelude.Control.Classes.
-Require Import Prelude.Control.Identity.
-Require Import Prelude.Equality.
+(** * Definition *)
 
-Local Close Scope nat_scope.
-Local Open Scope prelude_scope.
-
-(** * Definition
-
- *)
-
-Definition StateT
-           (s:  Type)
-           (m:  Type -> Type) `{Monad m}
-           (a:  Type)
-  : Type :=
+Definition state_t (s : Type) (m : Type -> Type) (a : Type) : Type :=
   s -> m (a * s).
 
-Definition runStateT
-           {m:    Type -> Type} `{Monad m}
-           {s a:  Type}
-           (ps:   StateT s m a)
-           (x:    s)
-  : m (a * s) :=
-  ps x.
+Bind Scope monad_scope with state_t.
 
-Definition evalStateT
-           {m:    Type -> Type} `{Monad m}
-           {s a:  Type}
-           (ps:   StateT s m a)
-           (x:    s)
-  : m a :=
-  fst <$> runStateT ps x.
+Definition run_state_t {m s a} (r : state_t s m a) (x : s) : m (a * s) :=
+  r x.
 
-Definition execStateT
-           {m:    Type -> Type} `{Monad m}
-           {s a:  Type}
-           (ps:   StateT s m a)
-           (x:    s)
-  : m s :=
-  snd <$> runStateT ps x.
+Definition eval_state_t {m s a} `{Monad m} (r : state_t s m a) (x : s) : m a :=
+  map fst (r x).
 
-(** * State Monad
+Definition exec_state_t {m s a} `{Monad m} (r : state_t s m a) (x : s) : m s :=
+  map snd (r x).
 
- *)
+(** * State Monad *)
 
-Definition state_map
-           {m:    Type -> Type} `{Monad m}
-           {s:    Type}
-           (a b:  Type)
-           (f:    a -> b)
-           (fs:   StateT s m a)
-  : StateT s m b :=
-    fun s
-    => (fun o => (f (fst o), snd o)) <$> fs s.
+Definition state_map {m s} `{Monad m} {a b} (f : a -> b) (r : state_t s m a)
+  : state_t s m b :=
+  fun* x => (fun o => (f (fst o), snd o)) <$> r x.
 
-Lemma state_functor_identity
-      (m:   Type -> Type) `{Monad m}
-      {s:   Type} `{Equality s}
-      {a:   Type} `{Equality a}
-      (ps:  StateT s m a)
-  : state_map _ _ id ps == id ps.
+Lemma state_functor_identity {m s a} `{Monad m} `{Equality s} `{Equality a}
+  (r : state_t s m a)
+  : state_map id r == id r.
+
 Proof.
-  cbn.
-  unfold state_map.
   intros x.
-  assert (R1: (fun (o: a * s) => (id (fst o), snd o)) = id). {
-    apply functional_extensionality.
-    intro o; destruct o; reflexivity.
-  }
-  rewrite R1.
-  apply functor_identity.
+  unfold state_map.
+  rewrite bind_map.
+  match goal with
+  | |- context[bind _ ?f] =>
+    assert (R: f == @pure m _ _);  [ now intros [y st] | rewrite R; clear R]
+  end.
+  apply bind_right_identity.
 Qed.
 
-Lemma state_functor_composition_identity
-      (m:      Type -> Type) `{Monad m}
-      {s:      Type} `{Equality s}
-      {a b c:  Type} `{Equality c}
-      (u:      b -> c)
-      (v:      a -> b)
-      (ps:     StateT s m a)
-  : state_map _ _ (u <<< v) ps == ((state_map _ _ u) <<< (state_map _ _ v)) ps.
+Lemma state_functor_composition_identity {m s a b c} `{Monad m} `{Equality s} `{Equality c}
+  (u : b -> c) (v : a -> b) (r : state_t s m a)
+  : state_map (u <<< v) r == ((state_map u) <<< (state_map v)) r.
+
 Proof.
-  cbn.
+  intros st.
   unfold state_map.
-  intros x.
-  assert (R1: (fun o : a * s => ((v >>> u) (fst o), snd o))
-              = ((fun o : a * s => (v (fst o), snd o))
-                   >>> (fun o : b * s => (u (fst o), snd o)))). {
-    apply functional_extensionality.
-    intros y.
-    destruct y.
-    cbn.
-    assert (R2: ((fun o : a * s => (v (fst o), snd o)) >>> (fun o : b * s => (u (fst o), snd o)))
-                = (fun o => ((v >>> u) (fst o), snd o))). {
-      apply functional_extensionality.
-      intros z.
-      destruct z.
-      reflexivity.
-    }
-    rewrite R2.
-    reflexivity.
-  }
-  rewrite R1.
-  apply functor_composition_identity.
+  change (fun o => ((u <<< v) (fst o), snd o))
+    with ((fun o => (v (fst o), snd o)) >>> (fun o : b * s => (u (fst o), snd o))).
+  apply functor_map_identity.
 Qed.
 
-Instance state_Functor
-         (m:  Type -> Type) `{Monad m}
-         (s:  Type) `{Equality s}
-  : Functor (StateT s m) :=
-  { map := state_map
+#[program]
+Instance state_Functor (m :  Type -> Type) `{Monad m} (s : Type) `{Equality s}
+  : Functor (state_t s m) :=
+  { map := @state_map m s _
   }.
-Proof.
-  + apply state_functor_identity.
-  + apply state_functor_composition_identity.
+
+Next Obligation.
+  apply state_functor_identity.
 Defined.
 
-Definition state_apply
-           {m:    Type -> Type} `{Monad m}
-           {s:    Type}
-           (a b:  Type)
-           (f:    StateT s m (a -> b))
-           (fs:   StateT s m a)
-  : StateT s m b :=
-  fun x
-  => u <- f x                                                       ;
-     v <- fs (snd u)                                                ;
-     pure ((fst u) (fst v), snd v).
+Next Obligation.
+  apply state_functor_composition_identity.
+Defined.
 
-Definition state_pure
-           {m:  Type -> Type} `{Monad m}
-           {s:  Type}
-           (a:  Type)
-           (x:  a)
-  : StateT s m a :=
-  fun t
-  => pure (x, t).
+Definition state_apply {m s} `{Monad m} {a b}
+  (f : state_t s m (a -> b)) (fs : state_t s m a)
+  : state_t s m b :=
+  fun* x => do
+    let* u <- f x in
+    let* v <- fs (snd u) in
+    pure (fst u (fst v), snd v)
+  end.
 
-Lemma state_applicative_identity
-      {m:  Type -> Type} `{Monad m}
-      {s:  Type} `{Equality s}
-      {a:  Type} `{Equality a}
-      (v:  StateT s m a):
-  state_apply _ _ (state_pure (a -> a) id) v == v.
+Definition state_pure {m s} `{Monad m} {a} (x : a) : state_t s m a :=
+  fun* s => pure (x, s).
+
+Lemma state_applicative_identity {m s} `{Monad m} `{Equality s} {a} `{Equality a}
+  (v : state_t s m a):
+  state_apply (state_pure id) v == v.
+
 Proof.
-  cbn.
+  intros st.
   unfold state_apply.
-  intros x.
-  assert (R1: (u <- state_pure (a -> a) id x; v0 <- v (snd u); pure (fst u (fst v0), snd v0))
-              == (v0 <- v x; pure (id (fst v0), snd v0))). {
-    cbn.
-    unfold state_apply, state_pure, id.
-    rewrite monad_left_identity.
-    reflexivity.
-  }
-  rewrite R1.
+  unfold state_pure.
+  rewrite bind_left_identity.
+  cbn.
   unfold id.
-  assert (R2: (fun (v0: a * s) => pure (f:=m) (fst v0, snd v0))
-              = (fun v0 => pure v0)). {
+  match goal with |- context[bind _ ?f] => assert (R: f = fun v0 : a * s => pure v0) end;
+  [| rewrite R; clear R]. {
     apply functional_extensionality.
-    intro y.
-    destruct y.
-    reflexivity.
+    now intros [x st'].
   }
-  rewrite R2.
-  rewrite monad_right_identity.
-  reflexivity.
+  apply bind_right_identity.
 Qed.
 
-Lemma state_applicative_homomorphism
-      {m:    Type -> Type} `{Monad m}
-      {s:    Type} `{Equality s}
-      {a b:  Type} `{Equality b}
-      (v:    a -> b)
-      (x:    a)
-  : state_apply _ _ (state_pure _ v) (state_pure _ x) == (state_pure _ (v x): StateT s m b).
+Lemma state_applicative_homomorphism {m s} `{Monad m} `{Equality s} {a b} `{Equality b}
+  (v : a -> b) (x : a)
+  : state_apply (state_pure v) (state_pure x) == state_pure (m:=m) (s:=s) (v x).
+
 Proof.
   cbn.
+  intros st.
   unfold state_apply, state_pure.
-  intro y.
-  rewrite monad_left_identity.
-  cbn.
-  rewrite monad_left_identity.
-  cbn.
-  reflexivity.
+  now repeat rewrite bind_left_identity.
 Qed.
 
-Lemma state_applicative_interchange
-      (m:    Type -> Type) `{Monad m}
-      {s:    Type} `{Equality s}
-      (a b:  Type) `{Equality b}
-      (u:    StateT s m (a -> b))
-      (y:    a)
-  : state_apply _ _ u (state_pure a y)
-    == state_apply _ _ (state_pure ((a -> b) -> b) (fun z : a -> b => z y)) u.
+Lemma state_applicative_interchange {m s} `{Monad m} `{Equality s} {a b} `{Equality b}
+  (u : state_t s m (a -> b)) (y : a)
+  : state_apply u (state_pure y) == state_apply (state_pure (fun z : a -> b => z y)) u.
+
 Proof.
-  cbn.
-  intro x.
+  intro st.
   unfold state_apply, state_pure.
-  rewrite monad_left_identity.
+  rewrite bind_left_identity.
   cbn.
-  assert (R1: (fun (u0: ((a -> b) * s))
-               => (v <- pure (f:=m) (y, snd u0);
-                   pure (fst u0 (fst v), snd v)))
-             == (fun (v: ((a -> b) * s))
-                  => pure (f:=m) (fst v y, snd v))). {
-    cbn.
-    intros z.
-    rewrite monad_left_identity.
-    reflexivity.
-  }
-  rewrite R1.
-  reflexivity.
+  match goal with
+  | |- bind _ ?f == bind _ ?g =>
+    assert (R : f == g); [| now rewrite R ]
+  end.
+  intros [f st'].
+  now rewrite bind_left_identity.
 Qed.
 
-Instance state_Applicative
-         (m:  Type -> Type) `{Monad m}
-         (s:  Type) `{Equality s}
-  : Applicative (StateT s m) :=
-  { pure := state_pure
-  ; apply := state_apply
+#[program]
+Instance state_Applicative (m : Type -> Type) `{Monad m} (s : Type) `{Equality s}
+  : Applicative (state_t s m) :=
+  { pure := @state_pure m s _
+  ; apply := @state_apply m s _
   }.
-Proof.
-  + apply (@state_applicative_identity m H s H0).
-  + intros a b c C u v w.
-    cbn.
-    unfold state_apply, state_pure.
-    intro x.
-    assert (R1: (u0 <- pure (@compose a b c, x); v0 <- u (snd u0); pure (fst u0 (fst v0), snd v0))
-                == (v0 <- u (snd (@compose a b c, x)); pure (fst (compose, x) (fst v0), snd v0))). {
-      rewrite monad_left_identity.
-      reflexivity.
-    }
-    repeat rewrite monad_bind_associativity.
-    rewrite monad_left_identity.
-    repeat rewrite monad_bind_associativity.
-    cbn.
-    assert (R2: (fun x0
-                 => (x1 <- pure (compose (fst x0), snd x0);
-                     u0 <- (v0 <- v (snd x1); pure (fst x1 (fst v0), snd v0));
-                     v0 <- w (snd u0); pure (fst u0 (fst v0), snd v0)))
-                == (fun u0
-                    => v0 <- (u1 <- v (snd u0); v0 <- w (snd u1); pure (fst u1 (fst v0), snd v0));
-                       pure (fst u0 (fst v0), snd v0))). {
-      intros y.
-      repeat rewrite monad_left_identity.
-      repeat rewrite monad_bind_associativity.
-      cbn.
-      assert (R3: (fun x0
-                  => (u0 <- pure (fst y <<< fst x0, snd x0);
-                      v0 <- w (snd u0); pure (fst u0 (fst v0), snd v0)))
-                  == fun x0
-                     => (v0 <- (v0 <- w (snd x0); pure (fst x0 (fst v0), snd v0));
-                         pure (fst y (fst v0), snd v0))). {
-        cbn.
-        intros z.
-        repeat rewrite monad_left_identity.
-        repeat rewrite monad_bind_associativity.
-        cbn.
-        assert (R4: (fun (v0: a * s)
-                     => pure (f:=m) ((fst y <<< fst z) (fst v0), snd v0))
-                    == (fun x0
-                        => v0 <- pure (fst z (fst x0), snd x0); pure (fst y (fst v0), snd v0))). {
-          cbn.
-          intros q.
-          repeat rewrite monad_left_identity.
-          cbn.
-          unfold compose.
-          reflexivity.
-        }
-        apply monad_bind_morphism.
-        intros n.
-        rewrite monad_left_identity.
-        reflexivity.
-      }
-      rewrite (monad_bind_morphism _ _ _ R3).
-      reflexivity.
-    }
-    rewrite (monad_bind_morphism _ _ _ R2).
-    reflexivity.
-  + apply (@state_applicative_homomorphism m H s H0).
-  + apply (@state_applicative_interchange m H s H0).
-  + intros a b B g x.
-    cbn.
-    intros y.
-    unfold state_apply, state_pure.
-    rewrite monad_left_identity.
-    cbn.
-    unfold state_map.
-    remember (fun o : a * s => (g (fst o), snd o)) as f.
-    assert ((x y >>= (fun (v: a * s)
-                      => pure (f:=m) (g (fst v), snd v)))
-           == (x y >>= (fun v => pure (f v)))).
-    rewrite Heqf.
-    reflexivity.
-    rewrite H1.
-    apply monad_bind_map.
+
+Next Obligation.
+  apply state_applicative_identity.
 Defined.
 
-Definition state_bind
-           {m:    Type -> Type} `{Monad m}
-           {s:    Type}
-           (a b:  Type)
-           (fs:   StateT s m a)
-           (f:    a -> StateT s m b)
-  : StateT s m b :=
-  fun x
-  => u <- fs x                                                       ;
-     f (fst u) (snd u).
-
-Lemma state_bind_associativity
-      (m:      Type -> Type) `{Monad m}
-      {s:      Type} `{Equality s}
-      (a b c:  Type) `{Equality c}
-      (f:      StateT s m a)
-      (g:      a -> StateT s m b)
-      (h:      b -> StateT s m c)
-  : state_bind b c (state_bind a b f g) h
-    == state_bind a c f (fun x : a => state_bind b c (g x) h).
-Proof.
+Next Obligation.
+  unfold state_apply, state_pure.
+  repeat rewrite bind_associativity.
+  repeat rewrite bind_left_identity.
+  repeat rewrite bind_associativity.
   cbn.
+  match goal with
+  | |- bind _ ?f == bind _ ?g => assert (R: f == g); [| now rewrite R ]
+  end.
+  intros [f st'].
+  repeat rewrite bind_associativity.
+  repeat rewrite bind_left_identity.
+  repeat rewrite bind_associativity.
+  cbn.
+  match goal with
+  | |- bind _ ?f == bind _ ?g => assert (R: f == g); [| now rewrite R ]
+  end.
+  intros [g st''].
+  cbn.
+  repeat rewrite bind_associativity.
+  repeat rewrite bind_left_identity.
+  cbn.
+  match goal with
+  | |- bind _ ?f == bind _ ?g => assert (R: f == g); [| now rewrite R ]
+  end.
+  intros [h st'''].
+  cbn.
+  unfold compose.
+  repeat rewrite bind_left_identity.
+  cbn.
+  reflexivity.
+Defined.
+
+Next Obligation.
+  apply state_applicative_homomorphism.
+Defined.
+
+Next Obligation.
+  + apply state_applicative_interchange.
+Defined.
+
+Next Obligation.
+  unfold state_map, state_pure, state_apply.
+  rewrite bind_left_identity.
+  cbn.
+  now rewrite bind_map.
+Qed.
+
+Definition state_bind {m s} `{Monad m} {a b}
+  (r : state_t s m a) (f : a -> state_t s m b)
+  : state_t s m b :=
+  fun* x => do
+    let* u <- r x in
+    f (fst u) (snd u)
+  end.
+
+Lemma state_bind_associativity {m s} `{Monad m} `{Equality s} {a b c} `{Equality c}
+  (f : state_t s m a) (g : a -> state_t s m b) (h : b -> state_t s m c)
+  : state_bind (state_bind f g) h == state_bind f (fun x : a => state_bind (g x) h).
+Proof.
+  intros st.
   unfold state_bind.
-  intros x.
-  rewrite monad_bind_associativity.
+  rewrite bind_associativity.
   reflexivity.
 Qed.
 
-Instance state_Monad
-         (m: Type -> Type) `{Monad m}
-         (s: Type) `{Equality s}
-  : Monad (StateT s m) :=
-  { bind := state_bind
+#[program]
+Instance state_Monad (m : Type -> Type) `{Monad m} (s : Type) `{Equality s}
+  : Monad (state_t s m) :=
+  { bind := @state_bind m s _
   }.
-Proof.
-  + intros a b B x f.
-    cbn.
-    unfold state_bind, state_pure.
-    intros y.
-    rewrite monad_left_identity.
-    reflexivity.
-  + intros a A x.
-    cbn.
-    unfold state_bind, state_pure.
-    intros y.
-    assert (R1: (fun (u: (a * s)) => pure (f:=m) (fst u, snd u))
-                = fun (u: (a * s)) => pure u). {
-      apply functional_extensionality.
-      intros [z  z'].
-      reflexivity.
-    }
-    rewrite R1.
-    apply monad_right_identity.
-  + apply state_bind_associativity.
-  + intros a b B p f f' Heq.
-    cbn.
-    unfold state_bind.
-    intros x.
-    assert (R1: (fun u => f (fst u) (snd u))
-                == fun u => f' (fst u) (snd u)). {
-      cbn.
-      intros y.
-    apply Heq.
-    }
-    rewrite (monad_bind_morphism _ _ _ R1).
-    reflexivity.
-  + intros a b B x f.
-    unfold state_bind.
-    intros y.
-    apply monad_bind_map.
+
+Next Obligation.
+  unfold state_bind, state_pure.
+  now rewrite bind_left_identity.
 Defined.
 
-(** * Transformer Instance
+Next Obligation.
+  unfold state_bind, state_pure.
+  assert (R: (fun u : a * s => pure (fst u, snd u)) == fun u : a * s => pure (f:=m) u)
+    by  now intros [y st].
+  rewrite R.
+  now rewrite bind_right_identity.
+Defined.
 
- *)
+Next Obligation.
+  apply state_bind_associativity.
+Defined.
 
-Definition state_lift
-           (s:  Type)
-           (m:  Type -> Type) `{Monad m}
-           (a:  Type)
-           (x:  m a)
-  : StateT s m a :=
-  fun s
-  => o <- x                                                          ;
-     pure (o, s).
+Next Obligation.
+  unfold state_bind.
+  match goal with
+  | |- bind _ ?f == bind _ ?g =>
+    assert (R: f == g); [ now intros | rewrite R; clear R ]
+  end.
+  reflexivity.
+Defined.
 
-Instance state_MonadTrans
-         (s:  Type) `{Equality s}
-  : MonadTrans (StateT s) :=
-  { lift := state_lift s
+Next Obligation.
+  unfold state_map, state_bind.
+  rewrite bind_map.
+  reflexivity.
+Defined.
+
+(** * Transformer Instance *)
+
+Definition state_lift {m s} `{Monad m} {a} (x : m a) : state_t s m a :=
+  fun s => bind x (fun o => pure (o, s)).
+
+Instance state_MonadTrans (s : Type) `{Equality s} : MonadTrans (state_t s) :=
+  { lift := fun m H => @state_lift m s H
   }.
 
-(** * State Instance
+(** * State Instance *)
 
- *)
+Definition state_get {m s} `{Monad m} : state_t s m s :=
+  fun x => pure (x, x).
 
-Definition state_get
-           (m:  Type -> Type) `{Monad m}
-           (s:  Type)
-  : StateT s m s :=
-  fun x
-  => pure (x, x).
+Definition state_put {m s} `{Monad m} (x : s) : state_t s m unit :=
+  fun _ => pure (tt, x).
 
-Definition state_put
-           (m:  Type -> Type) `{Monad m}
-           (s:  Type)
-           (x:  s)
-  : StateT s m unit :=
-  fun _
-  => pure (tt, x).
-
-Instance state_StateMonad
-         (m:  Type -> Type) `{Monad m}
-         (s:  Type) `{Equality s}
-  : MonadState s (StateT s m) :=
-  { get := state_get m s
-  ; put := state_put m s
+Instance state_StateMonad (m : Type -> Type) `{Monad m} (s : Type) `{Equality s}
+  : MonadState s (state_t s m) :=
+  { get := @state_get m s _
+  ; put := @state_put m s _
   }.
 
-(** * Pure Monad State
+(** * Pure Monad State *)
 
- *)
-
-Definition State
-           (s: Type) :=
-  StateT s Identity.
+Definition state (s : Type) := state_t s id.
