theories/Control/Sum.v
@@ -1,0 +1,166 @@
+(* coq-prelude
+ * Copyright (C) 2018 ANSSI
+ *
+ * This program is free software: you can redistribute it and/or modify
+ * it under the terms of the GNU General Public License as published by
+ * the Free Software Foundation, either version 3 of the License, or
+ * (at your option) any later version.
+ *
+ * This program is distributed in the hope that it will be useful,
+ * but WITHOUT ANY WARRANTY; without even the implied warranty of
+ * MERCHANTABILITY or FITNESS FOR A PARTICULAR PURPOSE.  See the
+ * GNU General Public License for more details.
+ *
+ * You should have received a copy of the GNU General Public License
+ * along with this program. If not, see <http://www.gnu.org/licenses/>.
+ *)
+
+Generalizable All Variables.
+
+From Coq.Program Require Import Equality.
+From Coq Require Import Setoid.
+
+From Prelude Require Export Control Function Equality.
+
+#[local]
+Open Scope prelude_scope.
+
+Bind Scope monad_scope with sum.
+
+Inductive sum_equal `{Equality l, Equality r} : l + r -> l + r -> Prop :=
+| equal_left (x y : l) (equ : x == y) : sum_equal (inl x) (inl y)
+| equal_right (x y : r) (equ : x == y) : sum_equal (inr x) (inr y).
+
+#[program]
+Instance sum_equal_Equivalence `{Equality l, Equality r}
+  : Equivalence (sum_equal (l:=l) (r:=r)).
+
+Next Obligation.
+  intros [x|x]; constructor; reflexivity.
+Defined.
+
+Next Obligation.
+  intros [x|x] y equ; inversion equ; subst; constructor; now symmetry.
+Defined.
+
+Next Obligation.
+  intros x [y|y] z equ1 equ2;
+    inversion equ1; subst;
+      inversion equ2; subst;
+        constructor;
+        etransitivity; eauto.
+Defined.
+
+Instance sum_Equality `{Equality l, Equality r} : Equality (l + r) :=
+  { equal := sum_equal
+  }.
+
+Definition sum_map {l a b} (f : a -> b) (x : l + a) : l + b :=
+  match x with
+  | inr x => inr (f x)
+  | inl x => inl x
+  end.
+
+#[program]
+Instance sum_Functor `{Equality l} : Functor (sum l) :=
+  { map := @sum_map l
+  }.
+
+Next Obligation.
+  destruct x as [x|x]; reflexivity.
+Defined.
+
+Next Obligation.
+  destruct x as [x|x]; reflexivity.
+Defined.
+
+Definition sum_pure {l a} (x : a) : l + a :=
+  inr x.
+
+Definition sum_app {l a b} (f : l + (a -> b)) (x : l + a) : l + b :=
+  match f, x with
+  | inr f, inr x => inr (f x)
+  | inl e, _ | _, inl e => inl e
+  end.
+
+#[program]
+Instance sum_Applicative `{Equality l} : Applicative (sum l) :=
+  { pure  := @sum_pure l
+  ; apply := @sum_app l
+  }.
+
+Next Obligation.
+  destruct v as [x|x]; reflexivity.
+Defined.
+
+Next Obligation.
+  destruct u; destruct v; destruct w; reflexivity.
+Defined.
+
+Next Obligation.
+  reflexivity.
+Defined.
+
+Next Obligation.
+  destruct u; reflexivity.
+Defined.
+
+Next Obligation.
+  destruct x; reflexivity.
+Defined.
+
+Definition sum_bind {l a b} (x : l + a) (f : a -> l + b) : l + b :=
+  match x with
+  | inr x => f x
+  | inl x => inl x
+  end.
+
+#[program]
+Instance sum_Monad `{Equality l} : Monad (sum l) :=
+  { bind := @sum_bind l
+  }.
+
+Next Obligation.
+  reflexivity.
+Defined.
+
+Next Obligation.
+  destruct x; reflexivity.
+Defined.
+
+Next Obligation.
+  destruct f; reflexivity.
+Defined.
+
+Next Obligation.
+  destruct x.
+  + reflexivity.
+  + apply H1.
+Defined.
+
+Next Obligation.
+  reflexivity.
+Defined.
+
+(** * Why not [EitherT]
+
+    Because of the definition of [EitherT m] (it is basically a
+    wrapper arround [m (Either)]), we cannot prove the functor laws
+    (and probably the other laws too).
+
+    In order to be able to prove these laws, we need an additionnal
+    law that tells [map f] is a morphism as long as [f] is a
+    morphism. This works pretty great with all monads defined in
+    [FreeSpec.Control], expect... [Program] (which is
+    unfortunate). The reason is the definition of the [Program]
+    [Equality] instance is too strong and require the results of the
+    realization of two equivalent programs to be equal, not
+    equivalent.
+
+    It is not clear how hard it would be to fix that, so for now we
+    have an ad-hoc solution. See the [FreeSpec.Fail] library for more
+    information about that. It basically provides the necessary tools
+    to promote an Interface so that the operational Semantics may
+    fail. It also provides a specific monad called [FailProgram] to
+    deal with the errors in a transparent manner.
+ *)
