theories/Data/Equality.v
@@ -1,0 +1,397 @@
+(* coq-prelude
+ * Copyright (C) 2018 ANSSI
+ *
+ * This program is free software: you can redistribute it and/or modify
+ * it under the terms of the GNU General Public License as published by
+ * the Free Software Foundation, either version 3 of the License, or
+ * (at your option) any later version.
+ *
+ * This program is distributed in the hope that it will be useful,
+ * but WITHOUT ANY WARRANTY; without even the implied warranty of
+ * MERCHANTABILITY or FITNESS FOR A PARTICULAR PURPOSE.  See the
+ * GNU General Public License for more details.
+ *
+ * You should have received a copy of the GNU General Public License
+ * along with this program. If not, see <http://www.gnu.org/licenses/>.
+ *)
+
+From Coq Require Import Setoid PeanoNat String Int63.
+From Prelude Require Import Init.
+
+(** * Equality
+
+    For a number of type, the Coq equality is too strong. Therefore,
+    we introduce the idea of a _weaker equality_ one can use in place
+    of the Leibniz equality used in Coq.
+
+ *)
+
+Class Equality (a : Type) :=
+  { equal (x y : a) : Prop
+  ; rel :> Equivalence equal
+  }.
+
+Arguments equal [a _] (_ _).
+
+(* To be used with [Proper] *)
+Notation "''equal'" := (@equal _ _) (only parsing) : prelude_scope.
+
+Instance default_Equality (a : Type)
+  : Equality a|999 :=
+  { equal := eq
+  }.
+
+Infix "==" := equal (at level 70, no associativity) : prelude_scope.
+Notation "x /= y" := (~ equal x y) (at level 70, no associativity) : prelude_scope.
+
+Lemma not_equal_sym
+      {A:    Type} `{Equality A}
+      (x y:  A)
+  : x /= y -> y /= x.
+Proof.
+  intros Hneq Heq.
+  now symmetry in Heq.
+Qed.
+
+Instance not_equal_Symmetric (A: Type) `{Equality A}
+  : Symmetric (fun x y => x /= y) :=
+  not_equal_sym.
+
+Class EquDec (a : Type) `{Equality a} :=
+  { equalb (x y : a) : bool
+  ; equalb_equ_true (x y : a) : x == y <-> equalb x y = true
+  }.
+
+Infix "?=" := equalb (at level 70, no associativity) : prelude_scope.
+Notation "x ?/= y" := (negb (x ?= y)) (at level 70, no associativity) : prelude_scope.
+
+Lemma equalb_equ_false `{EquDec a} (x y : a) : x /= y <-> x ?/= y = true.
+
+Proof.
+  case_eq (x ?= y); intros equ; cbn.
+  + rewrite <- equalb_equ_true in equ.
+    split.
+    ++ now intros equ'.
+    ++ now intros.
+  + split.
+    ++ auto.
+    ++ intros _.
+       intros falso.
+       rewrite equalb_equ_true in falso.
+       now rewrite equ in falso.
+Qed.
+
+(** * Instances *)
+
+(** ** Tactics *)
+
+(** We provide several tactics to easy the definition of [Equality]
+    and [DecidableEquality] instances. *)
+
+#[local]
+Ltac gen_default_decidable_equality a :=
+  match a with
+  | (?a == ?b /\ ?c)
+    => destruct (a ?= b); [ gen_default_decidable_equality c
+                          | now right
+                          ]
+  | ?a == ?b
+    => destruct (a ?= b); [ now left
+                          | now right
+                          ]
+  | _
+    => idtac
+  end.
+
+Ltac default_record_equality_instances :=
+  repeat constructor;
+    ( reflexivity
+    + (now symmetry)
+    + (repeat match goal with
+              | H: ?a /\ ?b |- _ => destruct H as [?A ?B]
+              end;
+       match goal with
+       | [H1: ?a == ?b, H2: ?b == ?c |- ?a == ?c]
+         => transitivity b; [exact H1 | exact H2]
+       | |- _
+         => idtac
+       end)
+    ).
+
+Ltac default_decidable_equality :=
+  match goal with
+  | |- { ?a } + { _ }
+    => gen_default_decidable_equality a
+  end.
+
+(** ** Function Instances *)
+
+#[program]
+Instance function_Equality {a} `{Equality b} : Equality (a -> b) :=
+  { equal := fun f g => forall (x: a), f x == g x
+  }.
+
+Next Obligation.
+  repeat constructor.
+  + now intro x.
+  + now intros x y.
+  + intros x y z H1 H2 r.
+    now etransitivity.
+Defined.
+
+(** ** Tuple Instances *)
+
+#[program]
+Instance tuple_Equality `{Equality a, Equality b} : Equality (a * b) :=
+  { equal := fun o o' => fst o == fst o' /\ snd o == snd o'
+  }.
+
+Next Obligation.
+  default_record_equality_instances.
+Defined.
+
+#[local] Open Scope signature_scope.
+From Coq Require Import Morphisms.
+
+Instance fst_tuple_equal_Proper `(Equality a, Equality b)
+  : Proper ('equal ==> 'equal) (@fst a b).
+
+Proof.
+  add_morphism_tactic.
+  intros o o' [P Q].
+  exact P.
+Qed.
+
+Instance snd_tuple_equal_Proper `(Equality a, Equality b)
+  : Proper ('equal ==> 'equal) (@snd a b).
+
+Proof.
+  add_morphism_tactic.
+  intros o o' [P Q].
+  exact Q.
+Qed.
+
+Instance pair_tuple_equal_Proper `(Equality a, Equality b)
+  : Proper ('equal ==> 'equal ==> 'equal) (@pair a b).
+
+Proof.
+  add_morphism_tactic.
+  intros o o' Heq p p' Heq'.
+  constructor; [ exact Heq
+               | exact Heq'
+               ].
+Qed.
+
+Lemma equalb_false_equ `{EquDec a} (x y : a) : (x ?= y) = false <-> (x ?/= y) = true.
+
+Proof.
+  case_eq (x ?= y); intros equ; split; now intros.
+Qed.
+
+#[program]
+Instance tuple_EquDec `{EquDec a, EquDec b} : EquDec (a * b) :=
+  { equalb := fun x y => andb (fst x ?= fst y) (snd x ?= snd y)
+  }.
+
+Next Obligation.
+  cbn.
+  case_eq (a1 ?= a0); intros equ; case_eq (b1 ?= b0); intros equ'; cbn.
+  + rewrite <- equalb_equ_true in equ.
+    rewrite <- equalb_equ_true in equ'.
+    now repeat split.
+  + rewrite <- equalb_equ_true in equ.
+    rewrite equalb_false_equ in equ'.
+    rewrite <- equalb_equ_false in equ'.
+    split.
+    ++ now intros [_ falso].
+    ++ now intros falso.
+  + rewrite <- equalb_equ_true in equ'.
+    rewrite equalb_false_equ in equ.
+    rewrite <- equalb_equ_false in equ.
+    split.
+    ++ now intros [falso _].
+    ++ now intros falso.
+  + rewrite equalb_false_equ in equ.
+    rewrite equalb_false_equ in equ'.
+    rewrite <- equalb_equ_false in equ.
+    rewrite <- equalb_equ_false in equ'.
+    now repeat split.
+Defined.
+
+(** ** Nat *)
+
+#[program]
+Instance nat_EquDec : @EquDec nat _ :=
+  { equalb := Nat.eqb
+  }.
+
+Next Obligation.
+  now rewrite Nat.eqb_eq.
+Defined.
+
+(** ** Z *)
+
+From Coq Require Import ZArith.
+
+#[program]
+Instance Z_EquDec : EquDec Z :=
+  { equalb := Z.eqb
+  }.
+
+Next Obligation.
+  now rewrite Z.eqb_eq.
+Defined.
+
+(** ** Bool *)
+
+#[program]
+Instance bool_EquDec : EquDec bool :=
+  { equalb := Bool.eqb
+  }.
+
+Next Obligation.
+  now rewrite Bool.eqb_true_iff.
+Defined.
+
+(** ** Option *)
+
+Inductive option_equal  `{Equality a} : option a -> option a -> Prop :=
+| option_equal_some (x y : a) (equ : x == y)
+  : option_equal (Some x) (Some y)
+| option_equal_none
+  : option_equal None None.
+
+#[program]
+Instance option_Equality `(Equality a) : Equality (option a) :=
+  { equal := option_equal
+  }.
+
+Next Obligation.
+  repeat constructor.
+  + intros [x | ]; now constructor.
+  + intros [x | ] y Heq; inversion Heq; subst; now constructor.
+  + intros x y z Heq Heq'.
+    inversion Heq; subst;
+      inversion Heq'; subst;
+        constructor.
+    now transitivity y0.
+Defined.
+
+Instance some_equal_Proper `(Equality a) : Proper ('equal ==> 'equal) (@Some a).
+
+Proof.
+  add_morphism_tactic.
+  intros x y Heq.
+  constructor.
+  exact Heq.
+Qed.
+
+(** ** List *)
+
+Inductive list_equal `{Equality a} : list a -> list a -> Prop :=
+| list_equal_cons (x y : a) (r r' :  list a) (equ : x == y) (next : list_equal r r')
+  : list_equal (x :: r) (y :: r')
+| list_equal_nil
+  : list_equal [] [].
+
+#[program]
+Instance list_Equality `(Equality a) : Equality (list a) :=
+  { equal := list_equal
+  }.
+
+Next Obligation.
+  repeat constructor.
+  + intros l; induction l; now constructor.
+  + intros l; induction l; intros l' Heq; inversion Heq; constructor.
+    ++ now subst.
+    ++ now apply IHl.
+  + intros l; induction l; intros l' l'' Heq Heq'; inversion Heq; subst; inversion Heq'; subst; constructor.
+    ++ now transitivity y.
+    ++ eapply IHl.
+       exact next.
+       exact next0.
+Defined.
+
+Fixpoint list_equal_dec `{EquDec a} (l l' : list a) : bool :=
+  match l, l' with
+  | [], [] => true
+  | x :: rst, y :: rst'
+    => andb (x ?= y) (list_equal_dec rst rst')
+  | _ :: _, []
+    => false
+  | [], _ :: _
+    => false
+  end.
+
+From Coq Require Import FunInd.
+Functional Scheme list_equal_dec_ind := Induction for list_equal_dec Sort Type.
+
+#[program]
+Instance list_EquDec
+         (a: Type) `{EquDec a}
+  : EquDec (list a) :=
+  { equalb := list_equal_dec
+  }.
+
+Next Obligation.
+  functional induction (list_equal_dec x y).
+  + repeat constructor.
+  + split.
+    ++ intros falso.
+       inversion falso.
+    ++ now intros.
+  + split.
+    ++ intros falso.
+       inversion falso.
+    ++ now intros.
+  + split.
+    ++ intros equ.
+       inversion equ; subst.
+       rewrite equalb_equ_true in equ0.
+       rewrite equ0.
+       now rewrite <- IHb.
+    ++ intros equ.
+       apply andb_prop in equ.
+       destruct equ as [equ1 equ2].
+       apply equalb_equ_true in equ1.
+       rewrite <- IHb in equ2.
+       now constructor.
+Defined.
+
+(** ** String *)
+
+#[program]
+Instance string_EquDec
+  : EquDec string :=
+  { equalb := String.eqb
+  }.
+
+Next Obligation.
+  now rewrite String.eqb_eq.
+Defined.
+
+(** ** Sigma-type *)
+
+#[program]
+Instance sigma_Equality `(Equality T) (P : T -> Prop)
+  : Equality { a: T | P a } :=
+  { equal := fun x y => proj1_sig x == proj1_sig y
+  }.
+
+Next Obligation.
+  default_record_equality_instances.
+  + now intro x.
+  + now intros x y.
+  + intros x y z Heq1 Heq2.
+    now transitivity (proj1_sig y).
+Defined.
+
+#[program]
+Instance sigma_EquDec `(EquDec T) (P : T -> Prop)
+  : EquDec { a: T | P a } :=
+  { equalb := fun x y => proj1_sig x ?= proj1_sig y
+  }.
+
+Next Obligation.
+  apply equalb_equ_true.
+Defined.
