theories/Init.v
@@ -1,0 +1,26 @@
+(* coq-prelude
+ * Copyright (C) 2018–2019 ANSSI
+ *
+ * This program is free software: you can redistribute it and/or modify
+ * it under the terms of the GNU General Public License as published by
+ * the Free Software Foundation, either version 3 of the License, or
+ * (at your option) any later version.
+ *
+ * This program is distributed in the hope that it will be useful,
+ * but WITHOUT ANY WARRANTY; without even the implied warranty of
+ * MERCHANTABILITY or FITNESS FOR A PARTICULAR PURPOSE.  See the
+ * GNU General Public License for more details.
+ *
+ * You should have received a copy of the GNU General Public License
+ * along with this program. If not, see <http://www.gnu.org/licenses/>.
+ *)
+
+Declare Scope prelude_scope.
+
+#[global] Open Scope prelude_scope.
+
+From Coq Require Export List.
+Export ListNotations.
+
+#[global]
+Generalizable All Variables.
